Pulse.Syntax.Printer: pretty-printing terms and st_terms

lib/steel/pulse/Pulse.Syntax.Printer.fst
@@ -8,6 +8,8 @@ module T = FStar.Tactics.V2
 module Un = FStar.Sealed
 module R = FStar.Reflection.V2
 
+module RU = Pulse.RuntimeUtils
+
 let tot_or_ghost_to_string = function
   | T.E_Total -> "total"
   | T.E_Ghost -> "ghost"
@@ -23,7 +25,7 @@ let dbg_printing : bool = true
 //   | Bool false -> "false"
 //   | Int i -> sprintf "%d" i
 
-let rec universe_to_string (n:nat) (u:universe) 
+let rec universe_to_string (n:nat) (u:universe)
   : Tot string (decreases u) =
   let open R in
   match inspect_universe u with
@@ -38,49 +40,14 @@ let rec universe_to_string (n:nat) (u:universe)
   | _ -> sprintf "<univ>"
 
 let univ_to_string u = sprintf "u#%s" (universe_to_string 0 u)
+let qual_to_doc = function
+  | None -> empty
+  | Some Implicit -> doc_of_string "#"
 let qual_to_string = function
   | None -> ""
   | Some Implicit -> "#"
 
 let indent (level:string) = level ^ "\t"
-    
-let rec term_to_string' (level:string) (t:term)
-  : T.Tac string
-  = match t.t with
-    | Tm_Emp -> "emp"
-
-    | Tm_Pure p ->
-      sprintf "pure (\n%s%s)" 
-        (indent level)
-        (term_to_string' (indent level) p)
-      
-    | Tm_Star p1 p2 ->
-      sprintf "%s ** \n%s%s" 
-        (term_to_string' level p1)
-        level
-        (term_to_string' level p2)
-                          
-    | Tm_ExistsSL _ b body ->
-      sprintf "(exists (%s:%s).\n%s%s)"
-              (T.unseal b.binder_ppname.name)
-              (term_to_string' (indent level) b.binder_ty)
-              level
-              (term_to_string' (indent level) body)
-
-    | Tm_ForallSL u b body ->
-      sprintf "(forall (%s:%s).\n%s%s)"
-              (T.unseal b.binder_ppname.name)
-              (term_to_string' (indent level) b.binder_ty)
-              level
-              (term_to_string' (indent level) body)
-                          
-    | Tm_VProp -> "vprop"
-    | Tm_Inames -> "inames"
-    | Tm_EmpInames -> "emp_inames"
-    | Tm_Unknown -> "_"
-    | Tm_FStar t ->
-      T.term_to_string t
-let term_to_string t = term_to_string' "" t
 
 let rec term_to_doc t
   : T.Tac document
@@ -94,30 +61,40 @@ let rec term_to_doc t
                 (term_to_doc p2)
 
     | Tm_ExistsSL _ b body ->
-      parens (doc_of_string "exists" ^/^ parens (doc_of_string (T.unseal b.binder_ppname.name)
-                                                  ^^ doc_of_string ":"
-                                                  ^^ term_to_doc b.binder_ty)
-              ^^ doc_of_string "."
-              ^/^ term_to_doc body)
+      prefix 2 1 (
+        group (prefix 2 1 (doc_of_string "exists")
+                            (parens (doc_of_string (T.unseal b.binder_ppname.name)
+                                                    ^^ doc_of_string ":"
+                                                    ^^ term_to_doc b.binder_ty)))
+                ^^ doc_of_string ".")
+        (term_to_doc body)
 
     | Tm_ForallSL u b body ->
-      parens (doc_of_string "forall" ^/^ parens (doc_of_string (T.unseal b.binder_ppname.name)
-                                                  ^^ doc_of_string ":"
-                                                  ^^ term_to_doc b.binder_ty)
-              ^^ doc_of_string "."
-              ^/^ term_to_doc body)
+      prefix 2 1 (
+        group (prefix 2 1 (doc_of_string "forall")
+                            (parens (doc_of_string (T.unseal b.binder_ppname.name)
+                                                    ^^ doc_of_string ":"
+                                                    ^^ term_to_doc b.binder_ty)))
+                ^^ doc_of_string ".")
+        (term_to_doc body)
 
     | Tm_VProp -> doc_of_string "vprop"
     | Tm_Inames -> doc_of_string "inames"
     | Tm_EmpInames -> doc_of_string "emp_inames"
+
     | Tm_Unknown -> doc_of_string "_"
     | Tm_FStar t ->
-      // Should call term_to_doc when available
-      doc_of_string (T.term_to_string t)
+      T.term_to_doc t
+
+let term_to_string t = render (term_to_doc t)
+
+let binder_to_doc (b:binder)
+  : T.Tac document
+  = doc_of_string (T.unseal b.binder_ppname.name) ^^ doc_of_string ":" ^^ term_to_doc b.binder_ty
 
 let binder_to_string (b:binder)
   : T.Tac string
-  = sprintf "%s:%s" 
+  = sprintf "%s:%s"
             (T.unseal b.binder_ppname.name)
             (term_to_string b.binder_ty)
 
@@ -126,31 +103,38 @@ let ctag_to_string = function
   | STT_Atomic -> "STAtomic"
   | STT_Ghost -> "STGhost"
 
-let comp_to_string (c:comp)
-  : T.Tac string
+// FIXME: track whether parentheses are needed. Or can we somehow detect
+// if a doc is atomic?
+let comp_to_doc (c:comp)
+  : T.Tac document
   = match c with
-    | C_Tot t -> 
-      sprintf "Tot %s" (term_to_string t)
-      
+    | C_Tot t ->
+      nest 2 (
+      doc_of_string "Tot" ^/^ term_to_doc t
+      )
+
     | C_ST s ->
-      sprintf "stt %s (requires\n%s) (ensures\n%s)"
-              (term_to_string s.res)
-              (term_to_string s.pre)
-              (term_to_string s.post)
+      nest 2 (
+      group (doc_of_string "stt" ^/^ term_to_doc s.res)
+      ^/^ nest 2 (group (parens (doc_of_string "requires" ^/^ term_to_doc s.pre)))
+      ^/^ nest 2 (group (parens (doc_of_string "ensures" ^/^ term_to_doc s.post)))
+      )
 
     | C_STAtomic inames s ->
-      sprintf "stt_atomic %s %s (requires\n%s) (ensures\n%s)"
-              (term_to_string inames)
-              (term_to_string s.res)
-              (term_to_string s.pre)
-              (term_to_string s.post)
+      nest 2 (
+      group (doc_of_string "stt_atomic" ^/^ term_to_doc inames ^/^ term_to_doc s.res)
+      ^/^ group (parens (doc_of_string "requires" ^/^ term_to_doc s.pre))
+      ^/^ group (parens (doc_of_string "ensures" ^/^ term_to_doc s.post))
+      )
 
     | C_STGhost inames s ->
-      sprintf "stt_atomic %s %s (requires\n%s) (ensures\n%s)"
-              (term_to_string inames)
-              (term_to_string s.res)
-              (term_to_string s.pre)
-              (term_to_string s.post)
+      nest 2 (
+      group (doc_of_string "stt_ghost" ^/^ term_to_doc inames ^/^ term_to_doc s.res)
+      ^/^ nest 2 (group (parens (doc_of_string "requires" ^/^ term_to_doc s.pre)))
+      ^/^ nest 2 (group (parens (doc_of_string "ensures" ^/^ term_to_doc s.post)))
+      )
+
+let comp_to_string c = render (comp_to_doc c)
 
 let term_opt_to_string (t:option term)
   : T.Tac string
@@ -162,198 +146,170 @@ let term_list_to_string (sep:string) (t:list term)
   : T.Tac string
   = String.concat sep (T.map term_to_string t)
 
-let rec st_term_to_string' (level:string) (t:st_term)
-  : T.Tac string
+(* Need these since the combinators expect tot functions... *)
+let separate_map (sep:document) (f : 'a -> T.Tac document) (l : list 'a) : T.Tac document =
+  separate sep (T.map f l)
+
+let braced (d:document) : document =
+  surround 2 1 (doc_of_string "{") d (doc_of_string "}")
+
+let rec st_term_to_doc (t:st_term)
+  : T.Tac document
   = match t.term with
     | Tm_Return { ctag; insert_eq; term } ->
-      sprintf "return_%s%s %s"
-        (match ctag with
-         | STT -> "stt"
-         | STT_Atomic -> "stt_atomic"
-         | STT_Ghost -> "stt_ghost")
-        (if insert_eq then "" else "_noeq")
-        (term_to_string term)
-      
+      group (
+        doc_of_string (sprintf "return_%s%s"
+                          (match ctag with
+                          | STT -> "stt"
+                          | STT_Atomic -> "stt_atomic"
+                          | STT_Ghost -> "stt_ghost")
+                          (if insert_eq then "" else "_noeq"))
+        ^/^ term_to_doc term)
+
     | Tm_STApp {head; arg_qual; arg } ->
-      sprintf "(%s%s %s%s)"
-        (if dbg_printing then "<stapp>" else "")
-        (term_to_string head)
-        (qual_to_string arg_qual)
-        (term_to_string arg)
-        
+      parens (
+        (if dbg_printing then doc_of_string "<stapp>" else empty)
+        ^/^ term_to_doc head
+        ^/^ qual_to_doc arg_qual ^^ term_to_doc arg
+      )
+
     | Tm_Bind { binder; head; body } ->
-      // if T.unseal binder.binder_ppname.name = "_"
-      // then sprintf "%s;\n%s%s" 
-      //              (st_term_to_string' level head)
-      //              level
-      //              (st_term_to_string' level body)                   
-      // else (
-        sprintf "let %s = %s;\n%s%s"
-          (binder_to_string binder)      
-          (st_term_to_string' level head)
-          level
-          (st_term_to_string' level body)
-      // )
+      surround 2 1
+        (group (surround 2 1 (doc_of_string "let") (binder_to_doc binder) (doc_of_string "=")))
+        (st_term_to_doc head)
+        (doc_of_string "in")
+      ^/^ st_term_to_doc body
 
     | Tm_TotBind { head; binder; body } ->
-      sprintf "let tot %s = %s;\n%s%s"
-        (binder_to_string binder)
-        (term_to_string head)
-        level
-        (st_term_to_string' level body)
-  
+      surround 2 1
+        (group (surround 2 1 (doc_of_string "let tot") (binder_to_doc binder) (doc_of_string "=")))
+        (term_to_doc head)
+        (doc_of_string "in")
+      ^/^ st_term_to_doc body
+
     | Tm_Abs { b; q; ascription=c; body } ->
-      sprintf "(fun (%s%s)\n%s\n {\n%s%s\n}"
-              (qual_to_string q)
-              (binder_to_string b)
-              (comp_to_string c)
-              (indent level)
-              (st_term_to_string' (indent level) body)
+      group (doc_of_string "fun" ^/^ parens (qual_to_doc q ^^ binder_to_doc b))
+      ^/^ braced (st_term_to_doc body)
 
     | Tm_If { b; then_; else_ } ->
-      sprintf "if (%s)\n%s{\n%s%s\n%s}\n%selse\n%s{\n%s%s\n%s}"
-        (term_to_string b)
-        level
-        (indent level)
-        (st_term_to_string' (indent level) then_)
-        level
-        level
-        level
-        (indent level)
-        (st_term_to_string' (indent level) else_)
-        level
+      prefix 2 1 (doc_of_string "if" ) (parens (term_to_doc b))
+      ^/^ braced (st_term_to_doc then_)
+      ^/^ doc_of_string "else"
+      ^/^ braced (st_term_to_doc else_)
 
     | Tm_Match {sc; brs} ->
-      sprintf "match (%s) with %s"
-        (term_to_string sc)
-        (branches_to_string brs)
+      surround 2 1 (doc_of_string "match") (parens (term_to_doc sc)) (doc_of_string "with")
+      ^/^ braced (branches_to_doc brs)
 
     | Tm_IntroPure { p } ->
-      sprintf "introduce pure (\n%s%s)"
-        (indent level)
-        (term_to_string' (indent level) p)
+      prefix 2 1 (doc_of_string "introduce pure") (parens (term_to_doc p))
 
     | Tm_ElimExists { p } ->
-      sprintf "elim_exists %s"
-        (term_to_string p)
+      prefix 2 1 (doc_of_string "elim_exists") (parens (term_to_doc p))
 
     | Tm_IntroExists { p; witnesses } ->
-      sprintf "introduce\n%s%s\n%swith %s"
-        (indent level)
-        (term_to_string' (indent level) p)
-        level
-        (term_list_to_string " " witnesses)
+      prefix 2 1 (doc_of_string "introduce") (parens (term_to_doc p))
+      ^/^ doc_of_string "with" ^/^ separate_map (doc_of_string " ") term_to_doc witnesses
 
     | Tm_While { invariant; condition; body } ->
-      sprintf "while (%s)\n%sinvariant %s\n%s{\n%s%s\n%s}"
-        (st_term_to_string' level condition)
-        level
-        (term_to_string invariant)
-        level
-        (indent level)
-        (st_term_to_string' (indent level) body)
-        level
+      prefix 2 1 (doc_of_string "while") (parens (group (st_term_to_doc condition)))
+      ^/^ nest 2 (prefix 2 1 (doc_of_string "invariant") (term_to_doc invariant))
+      ^/^ braced (st_term_to_doc body)
 
     | Tm_Par { pre1; body1; post1; pre2; body2; post2 } ->
-      sprintf "par (<%s> (%s) <%s) (<%s> (%s) <%s)"
-        (term_to_string pre1)
-        (st_term_to_string' level body1)
-        (term_to_string post1)
-        (term_to_string pre2)
-        (st_term_to_string' level body2)
-        (term_to_string post2)
+      doc_of_string "par"
+      ^/^ parens (angles (term_to_doc pre1) ^/^
+                  parens (st_term_to_doc body1) ^/^
+                  angles (term_to_doc post1))
+      ^/^ parens (angles (term_to_doc pre2) ^/^
+                  parens (st_term_to_doc body2) ^/^
+                  angles (term_to_doc post2))
 
     | Tm_Rewrite { t1; t2 } ->
-       sprintf "rewrite %s %s"
-        (term_to_string t1)
-        (term_to_string t2)
+       doc_of_string "rewrite"
+        ^/^ term_to_doc t1
+        ^/^ doc_of_string "as"
+        ^/^ term_to_doc t2
 
     | Tm_WithLocal { binder; initializer; body } ->
-      sprintf "let mut %s = %s;\n%s%s"
-        (binder_to_string binder)
-        (term_to_string initializer)
-        level
-        (st_term_to_string' level body)
+      doc_of_string "let mut" ^/^ binder_to_doc binder ^/^ doc_of_string "="
+      ^/^ term_to_doc initializer ^/^ doc_of_string "in"
+      ^/^ nest 2 (st_term_to_doc body)
 
     | Tm_WithLocalArray { binder; initializer; length; body } ->
-      sprintf "let mut %s = [| %s; %s |]\n%s%s"
-        (binder_to_string binder)
-        (term_to_string initializer)
-        (term_to_string length)
-        level
-        (st_term_to_string' level body)
+      doc_of_string "let mut" ^/^ binder_to_doc binder ^/^ doc_of_string "="
+      ^/^ brackets (term_to_doc initializer ^/^ doc_of_string ";" ^/^ term_to_doc length)
+      ^/^ doc_of_string "in"
+      ^/^ nest 2 (st_term_to_doc body)
 
     | Tm_Admit { ctag; u; typ; post } ->
-      sprintf "%s<%s> %s%s"
-        (match ctag with
-         | STT -> "stt_admit"
-         | STT_Atomic -> "stt_atomic_admit"
-         | STT_Ghost -> "stt_ghost_admit")
-        (universe_to_string 0 u)
-        (term_to_string typ)
-        (match post with
-         | None -> ""
-         | Some post -> sprintf " %s" (term_to_string post))
+      doc_of_string (match ctag with
+                      | STT -> "stt_admit"
+                      | STT_Atomic -> "stt_atomic_admit"
+                      | STT_Ghost -> "stt_ghost_admit")
+      ^/^ angles (doc_of_string (universe_to_string 0 u))
+      ^/^ term_to_doc typ
+      ^/^ (match post with
+           | None -> empty
+           | Some post -> term_to_doc post)
 
-    | Tm_ProofHintWithBinders { binders; hint_type; t} ->
+    | Tm_ProofHintWithBinders { binders; hint_type; t } ->
       let with_prefix =
         match binders with
-        | [] -> ""
-        | _ -> sprintf "with %s." (String.concat " " (T.map binder_to_string binders))
+        | [] -> empty
+        | _ -> doc_of_string "with" ^^ separate_map (doc_of_string " ") binder_to_doc binders ^^ doc_of_string "."
       in
-      let names_to_string = function
-        | None -> ""
-        | Some l -> sprintf " [%s]" (String.concat "; " l)
+      let names_to_doc = function
+        | None -> empty
+        | Some l -> brackets (separate_map (doc_of_string "; ") (fun n -> doc_of_string n) l)
       in
-      let ht, p =
+      let doc =
         match hint_type with
-        | ASSERT { p } -> "assert", term_to_string p
-        | UNFOLD { names; p } -> sprintf "unfold%s" (names_to_string names), term_to_string p
-        | FOLD { names; p } -> sprintf "fold%s" (names_to_string names), term_to_string p
+        | ASSERT { p } ->
+           doc_of_string "assert" ^/^ term_to_doc p
+        | UNFOLD { names; p } ->
+            doc_of_string "unfold" ^/^ names_to_doc names ^/^ term_to_doc p
+        | FOLD { names; p } ->
+            doc_of_string "fold" ^/^ names_to_doc names ^/^ term_to_doc p
         | RENAME { pairs; goal } ->
-          sprintf "rewrite each %s"
-            (String.concat ", "
-              (T.map
-                (fun (x, y) -> sprintf "%s as %s" (term_to_string x) (term_to_string y))
-              pairs)),
-            (match goal with
-            | None -> ""
-            | Some t -> sprintf " in %s" (term_to_string t))
+            doc_of_string "rename each" ^/^
+            separate_map (doc_of_string ", ") (fun (x, y) -> term_to_doc x ^/^ doc_of_string "as" ^/^ term_to_doc y) pairs
+            ^/^ (match goal with
+                 | None -> empty
+                 | Some t -> doc_of_string "in" ^/^ term_to_doc t)
         | REWRITE { t1; t2 } ->
-          sprintf "rewrite %s as %s" (term_to_string t1) (term_to_string t2), ""
+          doc_of_string "rewrite" ^/^ term_to_doc t1 ^/^ doc_of_string "as" ^/^ term_to_doc t2
       in
-      sprintf "%s %s %s; %s" with_prefix ht p
-        (st_term_to_string' level t)
+      with_prefix ^/^ doc ^^ semi ^/^ st_term_to_doc t
 
-and branches_to_string brs : T.Tac _ =
+and branches_to_doc brs : T.Tac document =
   match brs with
-  | [] -> ""
-  | b::bs -> branch_to_string b ^ branches_to_string bs
+  | [] -> empty
+  | b::bs -> branch_to_doc b ^^ hardline ^^ branches_to_doc bs
 
-and branch_to_string br : T.Tac _ =
+and branch_to_doc (br:branch) : T.Tac document =
   let (pat, e) = br in
-  Printf.sprintf "{ %s -> %s }"
-    (pattern_to_string pat)
-    (st_term_to_string' "" e)
+  braced (
+    pattern_to_doc pat
+    ^/^ doc_of_string "->"
+    ^/^ nest 2 (st_term_to_doc e))
 
-and pattern_to_string (p:pattern) : T.Tac string = 
+and pattern_to_doc (p:pattern) : T.Tac document =
   match p with
   | Pat_Cons fv pats ->
-    Printf.sprintf "(%s %s)"
-      (String.concat "." fv.fv_name) 
-      (String.concat " " (T.map (fun (p, _) -> pattern_to_string p) pats))
+    doc_of_string (String.concat "." fv.fv_name)
+    ^/^ separate_map (doc_of_string " ") (fun (p, _) -> pattern_to_doc p) pats
   | Pat_Constant c ->
-    "<constant>"
+    doc_of_string "<constant>"
   | Pat_Var x _ ->
-    T.unseal x
+    doc_of_string (T.unseal x)
   | Pat_Dot_Term None ->
-    ""
+    empty
   | Pat_Dot_Term (Some t) ->
-    Printf.sprintf "(.??)" //%s)" (term_to_string t)
-    
+    doc_of_string "(.??)" //%s)" (term_to_string t)
 
-
-let st_term_to_string t = st_term_to_string' "" t
+let pattern_to_string p = render (pattern_to_doc p)
+let st_term_to_string t = render (st_term_to_doc t)
 
 let tag_of_term (t:term) =
   match t.t with
@@ -396,7 +352,7 @@ let tag_of_comp (c:comp) : T.Tac string =
     Printf.sprintf "Atomic %s" (term_to_string i)
   | C_STGhost i _ ->
     Printf.sprintf "Ghost %s" (term_to_string i)
-    
+
 let rec print_st_head (t:st_term)
   : Tot string (decreases t) =
   match t.term with
@@ -415,7 +371,7 @@ let rec print_st_head (t:st_term)
   | Tm_STApp { head = p } -> print_head p
   | Tm_IntroPure _ -> "IntroPure"
   | Tm_IntroExists _ -> "IntroExists"
-  | Tm_ElimExists _ -> "ElimExists"  
+  | Tm_ElimExists _ -> "ElimExists"
   | Tm_ProofHintWithBinders _ -> "AssertWithBinders"
 and print_head (t:term) =
   match t with
@@ -425,7 +381,7 @@ and print_head (t:term) =
   | _ -> "<pure term>"
 
 
-let rec print_skel (t:st_term) = 
+let rec print_skel (t:st_term) =
   match t.term with
   | Tm_Abs { body }  -> Printf.sprintf "(fun _ -> %s)" (print_skel body)
   | Tm_Return { term = p } -> print_head p
